theories/concurrent/spmc_queue.v
@@ -13,7 +13,7 @@ From caml5.concurrent Require Import
 Implicit Types v t : val.
 Implicit Types vs : list val.
 
-Record spmc_queue `{!heapGS Σ} := {
+Record spmc_queue `{!heapGS Σ} {unboxed : bool} := {
   spmc_queue_make : val ;
   spmc_queue_push : val ;
   spmc_queue_pop : val ;
@@ -70,9 +70,16 @@ Record spmc_queue `{!heapGS Σ} := {
       (∃ vs' v, ⌜vs = vs' ++ [v] ∧ o = SOMEV v⌝ ∗ spmc_queue_model t γ vs') |
       RET o; True
     >>> ;
+
+  spmc_queue_unboxed :
+    if unboxed then ∀ t γ ι,
+      spmc_queue_inv t γ ι -∗
+      ⌜val_is_unboxed t⌝
+    else
+      True ;
 }.
-#[global] Arguments spmc_queue _ {_} : assert.
-#[global] Arguments Build_spmc_queue {_ _ _ _ _ _ _ _ _ _ _ _ _} _ _ _ : assert.
+#[global] Arguments spmc_queue _ {_} _ : assert.
+#[global] Arguments Build_spmc_queue {_ _} _ {_ _ _ _ _ _ _ _ _ _ _} _ _ _ _ : assert.
 #[global] Existing Instance spmc_queue_inv_persistent.
 #[global] Existing Instance spmc_queue_model_timeless.
 #[global] Existing Instance spmc_queue_producer_timeless.
@@ -93,7 +100,7 @@ Proof.
 Qed.
 
 Section spmc_queue_of_mpmc_queue.
-  Context `{SpmcQueueOfMpmcQueueG Σ} (mpmc_queue : mpmc_queue Σ).
+  Context `{SpmcQueueOfMpmcQueueG Σ} {unboxed} (mpmc_queue : mpmc_queue Σ unboxed).
 
   Notation "γ .(base)" := γ.1
   ( at level 5
@@ -102,7 +109,7 @@ Section spmc_queue_of_mpmc_queue.
   ( at level 5
   ) : stdpp_scope.
 
-  Program Definition spmc_queue_of_mpmc_queue := {|
+  Program Definition spmc_queue_of_mpmc_queue : spmc_queue Σ unboxed := {|
     spmc_queue_make :=
       mpmc_queue.(mpmc_queue_make) ;
     spmc_queue_push :=
@@ -136,5 +143,8 @@ Section spmc_queue_of_mpmc_queue.
   Qed.
   Next Obligation.
     intros. apply mpmc_queue_pop_spec.
+  Qed.
+  Next Obligation.
+    destruct unboxed; last done. eauto using mpmc_queue.(mpmc_queue_unboxed).
   Qed.
 End spmc_queue_of_mpmc_queue.
