theories/concurrent/ws_bag.v
@@ -11,13 +11,15 @@ From caml5.lang Require Import
 From caml5.concurrent Require Export
   base.
 From caml5.concurrent Require Import
+  mpmc_stack
+  mpmc_queue
   spmc_stack
   spmc_queue
   ws_deque.
 
 Implicit Types v t : val.
 
-Record ws_bag `{!heapGS Σ} := {
+Record ws_bag `{!heapGS Σ} {unboxed : bool} := {
   ws_bag_make : val ;
   ws_bag_push : val ;
   ws_bag_pop : val ;
@@ -94,15 +96,22 @@ Record ws_bag `{!heapGS Σ} := {
       RET from_option (λ v, SOMEV v) NONEV o;
       from_option Ψ True o
     >>> ;
+
+  ws_bag_unboxed :
+    if unboxed then ∀ t γ ι Ψ,
+      ws_bag_inv t γ ι Ψ -∗
+      ⌜val_is_unboxed t⌝
+    else
+      True ;
 }.
-#[global] Arguments ws_bag _ {_} : assert.
-#[global] Arguments Build_ws_bag {_ _ _ _ _ _ _ _ _ _ _ _ _ _} _ _ _ _ _ : assert.
+#[global] Arguments ws_bag _ {_} _ : assert.
+#[global] Arguments Build_ws_bag {_ _} _ {_ _ _ _ _ _ _ _ _ _ _ _} _ _ _ _ _ _ : assert.
 #[global] Existing Instance ws_bag_inv_ne.
 #[global] Existing Instance ws_bag_inv_persistent.
 #[global] Existing Instance ws_bag_model_timeless.
 #[global] Existing Instance ws_bag_owner_timeless.
 
-#[global] Instance ws_bag_inv_proper `{!heapGS Σ} ws_bag t γ ι :
+#[global] Instance ws_bag_inv_proper `{!heapGS Σ} {unboxed} (ws_bag : ws_bag Σ unboxed) t γ ι :
   Proper (pointwise_relation val (≡) ==> (≡)) (ws_bag.(ws_bag_inv) t γ ι).
 Proof.
   intros Ψ1 Ψ2 HΨ.
@@ -111,9 +120,9 @@ Proof.
 Qed.
 
 Class WsBagOfWsDequeG Σ `{!heapGS Σ} := {
-  ws_bag_of_ws_deque_G_ctl_G : AuthExclG Σ (listO valO) ;
+  ws_bag_of_ws_deque_G_model_G : AuthExclG Σ (listO valO) ;
 }.
-#[local] Existing Instance ws_bag_of_ws_deque_G_ctl_G.
+#[local] Existing Instance ws_bag_of_ws_deque_G_model_G.
 
 Definition ws_bag_of_ws_deque_Σ := #[
   auth_excl_Σ (listO valO)
@@ -126,8 +135,11 @@ Proof.
 Qed.
 
 Section ws_bag_of_ws_deque.
-  Context `{WsBagOfWsDequeG Σ} (ws_deque : ws_deque Σ).
-  Implicit Types γ : ws_deque.(ws_deque_name) * gname.
+  Context `{WsBagOfWsDequeG Σ} {unboxed} (ws_deque : ws_deque Σ unboxed).
+
+  Definition ws_bag_of_ws_deque_name : Type :=
+    ws_deque.(ws_deque_name) * gname.
+  Implicit Types γ : ws_bag_of_ws_deque_name.
 
   Notation "γ .(base)" := γ.1
   ( at level 5
@@ -136,7 +148,7 @@ Section ws_bag_of_ws_deque.
   ( at level 5
   ) : stdpp_scope.
 
-  Notation ws_bag_of_ws_deque_meta_ctl := (nroot .@ "ctl").
+  Notation ws_bag_of_ws_deque_meta_model := (nroot .@ "model").
 
   Notation ws_bag_of_ws_deque_namespace_base ι := (ι .@ "base").
   Notation ws_bag_of_ws_deque_namespace_extra ι := (ι .@ "extra").
@@ -157,14 +169,14 @@ Section ws_bag_of_ws_deque.
       let: "o" := ws_deque.(ws_deque_steal) "t" in
       "o".
 
-  #[local] Definition ws_bag_of_ws_deque_ctl₁ γ vs :=
+  #[local] Definition ws_bag_of_ws_deque_model₁ γ vs :=
     auth_excl_frag γ.(extra) vs.
-  #[local] Definition ws_bag_of_ws_deque_ctl₂ γ vs :=
+  #[local] Definition ws_bag_of_ws_deque_model₂ γ vs :=
     auth_excl_auth γ.(extra) (DfracOwn 1) vs.
 
   #[local] Definition ws_bag_of_ws_deque_inv_inner γ Ψ : iProp Σ :=
     ∃ vs,
-    ws_bag_of_ws_deque_ctl₁ γ vs ∗
+    ws_bag_of_ws_deque_model₁ γ vs ∗
     [∗ list] v ∈ vs, Ψ v.
   #[local] Definition ws_bag_of_ws_deque_inv t γ ι Ψ : iProp Σ :=
     ws_deque.(ws_deque_inv) t γ.(base) (ws_bag_of_ws_deque_namespace_base ι) ∗
@@ -173,7 +185,7 @@ Section ws_bag_of_ws_deque.
   #[local] Definition ws_bag_of_ws_deque_model t γ sz : iProp Σ :=
     ∃ vs,
     ⌜sz = length vs⌝ ∗
-    ws_bag_of_ws_deque_ctl₂ γ vs ∗
+    ws_bag_of_ws_deque_model₂ γ vs ∗
     ws_deque.(ws_deque_model) t γ.(base) vs.
 
   #[local] Definition ws_bag_of_ws_deque_owner t γ :=
@@ -226,8 +238,8 @@ Section ws_bag_of_ws_deque.
     iIntros "%Φ _ HΦ".
     iApply wp_fupd.
     wp_apply (ws_deque_make_spec with "[//]"). iIntros "%t %γ_base (#Hinv_deque & Hmodel_deque & Howner)".
-    iMod (auth_excl_alloc' []) as "(%γ_extra & Hctl₂ & Hctl₁)".
-    iApply ("HΦ" $! t (γ_base, γ_extra)). iFrame. iSplitL "Hctl₁".
+    iMod (auth_excl_alloc' []) as "(%γ_extra & Hmodel₂ & Hmodel₁)".
+    iApply ("HΦ" $! t (γ_base, γ_extra)). iFrame. iSplitL "Hmodel₁".
     - iFrame "#". iApply inv_alloc. iNext. iExists []. iFrame. done.
     - iExists []. auto with iFrame.
   Qed.
@@ -248,18 +260,18 @@ Section ws_bag_of_ws_deque.
   Proof.
     iIntros "!> %Φ ((#Hinv_deque & #Hinv_extra) & Howner & Hv) HΦ".
     awp_apply (ws_deque_push_spec with "[$Hinv_deque $Howner]").
-    iInv "Hinv_extra" as "(%vs & >Hctl₁ & Hvs)".
+    iInv "Hinv_extra" as "(%vs & >Hmodel₁ & Hvs)".
     iApply (aacc_aupd_commit with "HΦ"); first solve_ndisj.
-    iIntros "%sz (%_vs & -> & Hctl₂ & Hmodel_deque)".
-    iDestruct (auth_excl_both_agree_L with "Hctl₂ Hctl₁") as %->.
+    iIntros "%sz (%_vs & -> & Hmodel₂ & Hmodel_deque)".
+    iDestruct (auth_excl_both_agree_L with "Hmodel₂ Hmodel₁") as %->.
     iAaccIntro with "Hmodel_deque".
-    - iIntros "Hmodel_deque !>". iSplitL "Hctl₂ Hmodel_deque".
+    - iIntros "Hmodel_deque !>". iSplitL "Hmodel₂ Hmodel_deque".
       { iExists vs. auto with iFrame. }
       iIntros "$ !>". iFrame. iExists vs. auto with iFrame.
     - set vs' := vs ++ [v].
       iIntros "Hmodel_deque".
-      iMod (auth_excl_update' vs' with "Hctl₂ Hctl₁") as "(Hctl₂ & Hctl₁)".
-      iModIntro. iSplitL "Hctl₂ Hmodel_deque".
+      iMod (auth_excl_update' vs' with "Hmodel₂ Hmodel₁") as "(Hmodel₂ & Hmodel₁)".
+      iModIntro. iSplitL "Hmodel₂ Hmodel_deque".
       { iExists vs'. rewrite app_length /=. auto with iFrame lia. }
       iIntros "$ !>". iExists vs'. auto with iFrame.
   Qed.
@@ -283,28 +295,28 @@ Section ws_bag_of_ws_deque.
     iIntros "!> %Φ ((#Hinv_deque & #Hinv_extra) & Howner) HΦ".
     wp_rec.
     awp_apply (ws_deque_pop_spec with "[$Hinv_deque $Howner]").
-    iInv "Hinv_extra" as "(%vs & >Hctl₁ & Hvs)".
+    iInv "Hinv_extra" as "(%vs & >Hmodel₁ & Hvs)".
     iApply (aacc_aupd_commit with "HΦ"); first solve_ndisj.
-    iIntros "%sz (%_vs & -> & Hctl₂ & Hmodel_deque)".
-    iDestruct (auth_excl_both_agree_L with "Hctl₂ Hctl₁") as %->.
+    iIntros "%sz (%_vs & -> & Hmodel₂ & Hmodel_deque)".
+    iDestruct (auth_excl_both_agree_L with "Hmodel₂ Hmodel₁") as %->.
     iAaccIntro with "Hmodel_deque".
-    - iIntros "Hmodel_deque !>". iSplitL "Hctl₂ Hmodel_deque".
+    - iIntros "Hmodel_deque !>". iSplitL "Hmodel₂ Hmodel_deque".
       { iExists vs. auto with iFrame. }
       iIntros "$ !>". iExists vs. auto with iFrame.
     - iIntros "%o [((-> & ->) & Hmodel_deque) | (%vs' & %v & (-> & ->) & Hmodel_deque)]".
-      + iModIntro. iExists None. iSplitL "Hctl₂ Hmodel_deque".
+      + iModIntro. iExists None. iSplitL "Hmodel₂ Hmodel_deque".
         { iLeft. iSplit; first done. iExists []. auto with iFrame. }
-        iIntros "HΦ !>". iFrame. iSplitL "Hctl₁ Hvs".
+        iIntros "HΦ !>". iFrame. iSplitL "Hmodel₁ Hvs".
         { iExists []. auto. }
         iIntros "Howner". wp_pures. iApply "HΦ". auto.
-      + iMod (auth_excl_update' vs' with "Hctl₂ Hctl₁") as "(Hctl₂ & Hctl₁)".
+      + iMod (auth_excl_update' vs' with "Hmodel₂ Hmodel₁") as "(Hmodel₂ & Hmodel₁)".
         iDestruct "Hvs" as "(Hvs' & Hv & _)".
-        iModIntro. iExists (Some v). iSplitL "Hctl₂ Hmodel_deque".
+        iModIntro. iExists (Some v). iSplitL "Hmodel₂ Hmodel_deque".
         { iRight. iExists (length vs'), v. iSplit.
           { rewrite app_length (comm Nat.add) //. }
           iExists vs'. auto with iFrame.
         }
-        iIntros "HΦ !>". iSplitL "Hctl₁ Hvs'".
+        iIntros "HΦ !>". iSplitL "Hmodel₁ Hvs'".
         { iExists vs'. auto with iFrame. }
         iIntros "Howner". wp_pures. iApply "HΦ". auto with iFrame.
   Qed.
@@ -326,44 +338,37 @@ Section ws_bag_of_ws_deque.
     iIntros "!> %Φ (#Hinv_deque & #Hinv_extra) HΦ".
     wp_rec.
     awp_apply (ws_deque_steal_spec with "Hinv_deque").
-    iInv "Hinv_extra" as "(%vs & >Hctl₁ & Hvs)".
+    iInv "Hinv_extra" as "(%vs & >Hmodel₁ & Hvs)".
     iApply (aacc_aupd_commit with "HΦ"); first solve_ndisj.
-    iIntros "%sz (%_vs & -> & Hctl₂ & Hmodel_deque)".
-    iDestruct (auth_excl_both_agree_L with "Hctl₂ Hctl₁") as %->.
+    iIntros "%sz (%_vs & -> & Hmodel₂ & Hmodel_deque)".
+    iDestruct (auth_excl_both_agree_L with "Hmodel₂ Hmodel₁") as %->.
     iAaccIntro with "Hmodel_deque".
-    - iIntros "Hmodel_deque !>". iSplitL "Hctl₂ Hmodel_deque".
+    - iIntros "Hmodel_deque !>". iSplitL "Hmodel₂ Hmodel_deque".
       { iExists vs. auto with iFrame. }
       iIntros "$ !>". iExists vs. auto with iFrame.
     - iIntros "%o [((-> & ->) & Hmodel_deque) | (%v & %vs' & (-> & ->) & Hmodel_deque)]".
-      + iModIntro. iExists None. iSplitL "Hctl₂ Hmodel_deque".
+      + iModIntro. iExists None. iSplitL "Hmodel₂ Hmodel_deque".
         { iLeft. iSplit; first done. iExists []. auto with iFrame. }
-        iIntros "HΦ !>". iFrame. iSplitL "Hctl₁ Hvs".
+        iIntros "HΦ !>". iFrame. iSplitL "Hmodel₁ Hvs".
         { iExists []. auto. }
         iIntros "Howner". wp_pures. iApply "HΦ". auto.
-      + iMod (auth_excl_update' vs' with "Hctl₂ Hctl₁") as "(Hctl₂ & Hctl₁)".
+      + iMod (auth_excl_update' vs' with "Hmodel₂ Hmodel₁") as "(Hmodel₂ & Hmodel₁)".
         iDestruct "Hvs" as "(Hv & Hvs')".
-        iModIntro. iExists (Some v). iSplitL "Hctl₂ Hmodel_deque".
+        iModIntro. iExists (Some v). iSplitL "Hmodel₂ Hmodel_deque".
         { iRight. iExists (length vs'), v. iSplit; first done.
           iExists vs'. auto with iFrame.
         }
-        iIntros "HΦ !>". iSplitL "Hctl₁ Hvs'".
+        iIntros "HΦ !>". iSplitL "Hmodel₁ Hvs'".
         { iExists vs'. auto with iFrame. }
         iIntros "Howner". wp_pures. iApply "HΦ". auto with iFrame.
   Qed.
-
-  Definition ws_bag_of_ws_deque :=
-    Build_ws_bag
-      ws_bag_of_ws_deque_owner_exclusive
-      ws_bag_of_ws_deque_make_spec
-      ws_bag_of_ws_deque_push_spec
-      ws_bag_of_ws_deque_pop_spec
-      ws_bag_of_ws_deque_steal_spec.
 End ws_bag_of_ws_deque.
 
+
 Class WsBagOfSpmcStackG Σ `{!heapGS Σ} := {
-  ws_bag_of_spmc_stack_G_ctl_G : AuthExclG Σ (listO valO) ;
+  ws_bag_of_spmc_stack_G_model_G : AuthExclG Σ (listO valO) ;
 }.
-#[local] Existing Instance ws_bag_of_spmc_stack_G_ctl_G.
+#[local] Existing Instance ws_bag_of_spmc_stack_G_model_G.
 
 Definition ws_bag_of_spmc_stack_Σ := #[
   auth_excl_Σ (listO valO)
@@ -376,8 +381,11 @@ Proof.
 Qed.
 
 Section ws_bag_of_spmc_stack.
-  Context `{WsBagOfSpmcStackG Σ} (spmc_stack : spmc_stack Σ).
-  Implicit Types γ : spmc_stack.(spmc_stack_name) * gname.
+  Context `{WsBagOfSpmcStackG Σ} {unboxed} (spmc_stack : spmc_stack Σ unboxed).
+
+  Definition ws_bag_of_spmc_stack_name : Type :=
+    spmc_stack.(spmc_stack_name) * gname.
+  Implicit Types γ : ws_bag_of_spmc_stack_name.
 
   Notation "γ .(base)" := γ.1
   ( at level 5
@@ -386,7 +394,7 @@ Section ws_bag_of_spmc_stack.
   ( at level 5
   ) : stdpp_scope.
 
-  Notation ws_bag_of_spmc_stack_meta_ctl := (nroot .@ "ctl").
+  Notation ws_bag_of_spmc_stack_meta_model := (nroot .@ "model").
 
   Notation ws_bag_of_spmc_stack_namespace_base ι := (ι .@ "base").
   Notation ws_bag_of_spmc_stack_namespace_extra ι := (ι .@ "extra").
@@ -407,14 +415,14 @@ Section ws_bag_of_spmc_stack.
       let: "o" := spmc_stack.(spmc_stack_pop) "t" in
       "o".
 
-  #[local] Definition ws_bag_of_spmc_stack_ctl₁ γ vs :=
+  #[local] Definition ws_bag_of_spmc_stack_model₁ γ vs :=
     auth_excl_frag γ.(extra) vs.
-  #[local] Definition ws_bag_of_spmc_stack_ctl₂ γ vs :=
+  #[local] Definition ws_bag_of_spmc_stack_model₂ γ vs :=
     auth_excl_auth γ.(extra) (DfracOwn 1) vs.
 
   #[local] Definition ws_bag_of_spmc_stack_inv_inner γ Ψ : iProp Σ :=
     ∃ vs,
-    ws_bag_of_spmc_stack_ctl₁ γ vs ∗
+    ws_bag_of_spmc_stack_model₁ γ vs ∗
     [∗ list] v ∈ vs, Ψ v.
   #[local] Definition ws_bag_of_spmc_stack_inv t γ ι Ψ : iProp Σ :=
     spmc_stack.(spmc_stack_inv) t γ.(base) (ws_bag_of_spmc_stack_namespace_base ι) ∗
@@ -423,7 +431,7 @@ Section ws_bag_of_spmc_stack.
   #[local] Definition ws_bag_of_spmc_stack_model t γ sz : iProp Σ :=
     ∃ vs,
     ⌜sz = length vs⌝ ∗
-    ws_bag_of_spmc_stack_ctl₂ γ vs ∗
+    ws_bag_of_spmc_stack_model₂ γ vs ∗
     spmc_stack.(spmc_stack_model) t γ.(base) vs.
 
   #[local] Definition ws_bag_of_spmc_stack_owner t γ :=
@@ -476,8 +484,8 @@ Section ws_bag_of_spmc_stack.
     iIntros "%Φ _ HΦ".
     iApply wp_fupd.
     wp_apply (spmc_stack_make_spec with "[//]"). iIntros "%t %γ_deque (#Hinv_deque & Hmodel_deque & Howner)".
-    iMod (auth_excl_alloc' []) as "(%γ_extra & Hctl₂ & Hctl₁)".
-    iApply ("HΦ" $! t (γ_deque, γ_extra)). iFrame. iSplitL "Hctl₁".
+    iMod (auth_excl_alloc' []) as "(%γ_extra & Hmodel₂ & Hmodel₁)".
+    iApply ("HΦ" $! t (γ_deque, γ_extra)). iFrame. iSplitL "Hmodel₁".
     - iFrame "#". iApply inv_alloc. iNext. iExists []. iFrame. done.
     - iExists []. auto with iFrame.
   Qed.
@@ -498,18 +506,18 @@ Section ws_bag_of_spmc_stack.
   Proof.
     iIntros "!> %Φ ((#Hinv_deque & #Hinv_extra) & Howner & Hv) HΦ".
     awp_apply (spmc_stack_push_spec with "[$Hinv_deque $Howner]").
-    iInv "Hinv_extra" as "(%vs & >Hctl₁ & Hvs)".
+    iInv "Hinv_extra" as "(%vs & >Hmodel₁ & Hvs)".
     iApply (aacc_aupd_commit with "HΦ"); first solve_ndisj.
-    iIntros "%sz (%_vs & -> & Hctl₂ & Hmodel_deque)".
-    iDestruct (auth_excl_both_agree_L with "Hctl₂ Hctl₁") as %->.
+    iIntros "%sz (%_vs & -> & Hmodel₂ & Hmodel_deque)".
+    iDestruct (auth_excl_both_agree_L with "Hmodel₂ Hmodel₁") as %->.
     iAaccIntro with "Hmodel_deque".
-    - iIntros "Hmodel_deque !>". iSplitL "Hctl₂ Hmodel_deque".
+    - iIntros "Hmodel_deque !>". iSplitL "Hmodel₂ Hmodel_deque".
       { iExists vs. auto with iFrame. }
       iIntros "$ !>". iFrame. iExists vs. auto with iFrame.
     - set vs' := v :: vs.
       iIntros "Hmodel_deque".
-      iMod (auth_excl_update' vs' with "Hctl₂ Hctl₁") as "(Hctl₂ & Hctl₁)".
-      iModIntro. iSplitL "Hctl₂ Hmodel_deque".
+      iMod (auth_excl_update' vs' with "Hmodel₂ Hmodel₁") as "(Hmodel₂ & Hmodel₁)".
+      iModIntro. iSplitL "Hmodel₂ Hmodel_deque".
       { iExists vs'. auto with iFrame. }
       iIntros "$ !>". iExists vs'. auto with iFrame.
   Qed.
@@ -533,27 +541,27 @@ Section ws_bag_of_spmc_stack.
     iIntros "!> %Φ ((#Hinv_deque & #Hinv_extra) & Howner) HΦ".
     wp_rec.
     awp_apply (spmc_stack_pop_spec with "Hinv_deque").
-    iInv "Hinv_extra" as "(%vs & >Hctl₁ & Hvs)".
+    iInv "Hinv_extra" as "(%vs & >Hmodel₁ & Hvs)".
     iApply (aacc_aupd_commit with "HΦ"); first solve_ndisj.
-    iIntros "%sz (%_vs & -> & Hctl₂ & Hmodel_deque)".
-    iDestruct (auth_excl_both_agree_L with "Hctl₂ Hctl₁") as %->.
+    iIntros "%sz (%_vs & -> & Hmodel₂ & Hmodel_deque)".
+    iDestruct (auth_excl_both_agree_L with "Hmodel₂ Hmodel₁") as %->.
     iAaccIntro with "Hmodel_deque".
-    - iIntros "Hmodel_deque !>". iSplitL "Hctl₂ Hmodel_deque".
+    - iIntros "Hmodel_deque !>". iSplitL "Hmodel₂ Hmodel_deque".
       { iExists vs. auto with iFrame. }
       iIntros "$ !>". iFrame. iExists vs. iFrame.
     - iIntros "%o [((-> & ->) & Hmodel_deque) | (%v & %vs' & (-> & ->) & Hmodel_deque)]".
-      + iModIntro. iExists None. iSplitL "Hctl₂ Hmodel_deque".
+      + iModIntro. iExists None. iSplitL "Hmodel₂ Hmodel_deque".
         { iLeft. iSplit; first done. iExists []. auto with iFrame. }
-        iIntros "HΦ !>". iFrame. iSplitL "Hctl₁ Hvs".
+        iIntros "HΦ !>". iFrame. iSplitL "Hmodel₁ Hvs".
         { iExists []. auto. }
         iIntros "_". wp_pures. iApply "HΦ". auto with iFrame.
-      + iMod (auth_excl_update' vs' with "Hctl₂ Hctl₁") as "(Hctl₂ & Hctl₁)".
+      + iMod (auth_excl_update' vs' with "Hmodel₂ Hmodel₁") as "(Hmodel₂ & Hmodel₁)".
         iDestruct "Hvs" as "(Hv & Hvs')".
-        iModIntro. iExists (Some v). iSplitL "Hctl₂ Hmodel_deque".
+        iModIntro. iExists (Some v). iSplitL "Hmodel₂ Hmodel_deque".
         { iRight. iExists (length vs'), v. iSplit; first done.
           iExists vs'. auto with iFrame.
         }
-        iIntros "HΦ !>". iSplitL "Hctl₁ Hvs'".
+        iIntros "HΦ !>". iSplitL "Hmodel₁ Hvs'".
         { iExists vs'. auto with iFrame. }
         iIntros "_". wp_pures. iApply "HΦ". auto with iFrame.
   Qed.
@@ -575,44 +583,97 @@ Section ws_bag_of_spmc_stack.
     iIntros "!> %Φ (#Hinv_deque & #Hinv_extra) HΦ".
     wp_rec.
     awp_apply (spmc_stack_pop_spec with "Hinv_deque").
-    iInv "Hinv_extra" as "(%vs & >Hctl₁ & Hvs)".
+    iInv "Hinv_extra" as "(%vs & >Hmodel₁ & Hvs)".
     iApply (aacc_aupd_commit with "HΦ"); first solve_ndisj.
-    iIntros "%sz (%_vs & -> & Hctl₂ & Hmodel_deque)".
-    iDestruct (auth_excl_both_agree_L with "Hctl₂ Hctl₁") as %->.
+    iIntros "%sz (%_vs & -> & Hmodel₂ & Hmodel_deque)".
+    iDestruct (auth_excl_both_agree_L with "Hmodel₂ Hmodel₁") as %->.
     iAaccIntro with "Hmodel_deque".
-    - iIntros "Hmodel_deque !>". iSplitL "Hctl₂ Hmodel_deque".
+    - iIntros "Hmodel_deque !>". iSplitL "Hmodel₂ Hmodel_deque".
       { iExists vs. auto with iFrame. }
       iIntros "$ !>". iExists vs. auto with iFrame.
     - iIntros "%o [((-> & ->) & Hmodel_deque) | (%v & %vs' & (-> & ->) & Hmodel_deque)]".
-      + iModIntro. iExists None. iSplitL "Hctl₂ Hmodel_deque".
+      + iModIntro. iExists None. iSplitL "Hmodel₂ Hmodel_deque".
         { iLeft. iSplit; first done. iExists []. auto with iFrame. }
-        iIntros "HΦ !>". iFrame. iSplitL "Hctl₁ Hvs".
+        iIntros "HΦ !>". iFrame. iSplitL "Hmodel₁ Hvs".
         { iExists []. auto. }
         iIntros "_". wp_pures. iApply "HΦ". auto.
-      + iMod (auth_excl_update' vs' with "Hctl₂ Hctl₁") as "(Hctl₂ & Hctl₁)".
+      + iMod (auth_excl_update' vs' with "Hmodel₂ Hmodel₁") as "(Hmodel₂ & Hmodel₁)".
         iDestruct "Hvs" as "(Hv & Hvs')".
-        iModIntro. iExists (Some v). iSplitL "Hctl₂ Hmodel_deque".
+        iModIntro. iExists (Some v). iSplitL "Hmodel₂ Hmodel_deque".
         { iRight. iExists (length vs'), v. iSplit; first done.
           iExists vs'. auto with iFrame.
         }
-        iIntros "HΦ !>". iSplitL "Hctl₁ Hvs'".
+        iIntros "HΦ !>". iSplitL "Hmodel₁ Hvs'".
         { iExists vs'. auto with iFrame. }
         iIntros "_". wp_pures. iApply "HΦ". auto with iFrame.
   Qed.
-
-  Definition ws_bag_of_spmc_stack :=
-    Build_ws_bag
-      ws_bag_of_spmc_stack_owner_exclusive
-      ws_bag_of_spmc_stack_make_spec
-      ws_bag_of_spmc_stack_push_spec
-      ws_bag_of_spmc_stack_pop_spec
-      ws_bag_of_spmc_stack_steal_spec.
 End ws_bag_of_spmc_stack.
 
-Class WsBagOfSpmcQueueG Σ `{!heapGS Σ} := {
-  ws_bag_of_spmc_queue_G_ctl_G : AuthExclG Σ (listO valO) ;
+#[local] Lemma ws_bag_of_spmc_stack_unboxed `{WsBagOfSpmcStackG Σ} {unboxed} (spmc_stack : spmc_stack Σ unboxed) :
+  if unboxed then ∀ t γ ι Ψ,
+    ws_bag_of_spmc_stack_inv spmc_stack t γ ι Ψ -∗
+    ⌜val_is_unboxed t⌝
+  else
+    True.
+Proof.
+  destruct unboxed; last done.
+  iIntros "%t %γ %ι %Ψ (#Hinv_deque & #Hinv_extra)".
+  iApply (spmc_stack.(spmc_stack_unboxed) with "Hinv_deque").
+Qed.
+
+Definition ws_bag_of_spmc_stack `{WsBagOfSpmcStackG Σ} {unboxed} (spmc_stack : spmc_stack Σ unboxed) : ws_bag Σ unboxed := {|
+  ws_bag_make := ws_bag_of_spmc_stack_make spmc_stack ;
+  ws_bag_push := ws_bag_of_spmc_stack_push spmc_stack ;
+  ws_bag_pop := ws_bag_of_spmc_stack_pop spmc_stack ;
+  ws_bag_steal := ws_bag_of_spmc_stack_steal spmc_stack ;
+
+  ws_bag_name := ws_bag_of_spmc_stack_name spmc_stack ;
+  ws_bag_inv := ws_bag_of_spmc_stack_inv spmc_stack ;
+  ws_bag_model := ws_bag_of_spmc_stack_model spmc_stack ;
+  ws_bag_owner := ws_bag_of_spmc_stack_owner spmc_stack ;
+
+  ws_bag_inv_ne := ws_bag_of_spmc_stack_inv_ne spmc_stack ;
+  ws_bag_inv_persistent := ws_bag_of_spmc_stack_inv_persistent spmc_stack ;
+  ws_bag_model_timeless := ws_bag_of_spmc_stack_model_timeless spmc_stack ;
+  ws_bag_owner_timeless := ws_bag_of_spmc_stack_owner_timeless spmc_stack ;
+
+  ws_bag_owner_exclusive := ws_bag_of_spmc_stack_owner_exclusive spmc_stack ;
+
+  ws_bag_make_spec := ws_bag_of_spmc_stack_make_spec spmc_stack ;
+  ws_bag_push_spec := ws_bag_of_spmc_stack_push_spec spmc_stack ;
+  ws_bag_pop_spec := ws_bag_of_spmc_stack_pop_spec spmc_stack ;
+  ws_bag_steal_spec := ws_bag_of_spmc_stack_steal_spec spmc_stack ;
+
+  ws_bag_unboxed := ws_bag_of_spmc_stack_unboxed spmc_stack ;
+|}.
+
+Class WsBagOfMpmcStackG Σ `{!heapGS Σ} := {
+  ws_bag_of_mpmc_stack_G_mpmc_stack_G : SpmcStackOfMpmcStackG Σ ;
+  ws_bag_of_mpmc_stack_G_spmc_stack_G : WsBagOfSpmcStackG Σ ;
 }.
-#[local] Existing Instance ws_bag_of_spmc_queue_G_ctl_G.
+#[local] Existing Instance ws_bag_of_mpmc_stack_G_mpmc_stack_G.
+#[local] Existing Instance ws_bag_of_mpmc_stack_G_spmc_stack_G.
+
+Definition ws_bag_of_mpmc_stack_Σ := #[
+  spmc_stack_of_mpmc_stack_Σ ;
+  ws_bag_of_spmc_stack_Σ
+].
+Lemma subG_ws_bag_of_mpmc_stack_Σ Σ `{!heapGS Σ} :
+  subG ws_bag_of_mpmc_stack_Σ Σ →
+  WsBagOfMpmcStackG Σ.
+Proof.
+  pose subG_spmc_stack_of_mpmc_stack_Σ.
+  pose subG_ws_bag_of_spmc_stack_Σ.
+  solve_inG.
+Qed.
+
+Definition ws_bag_of_mpmc_stack `{WsBagOfMpmcStackG Σ} {unboxed} (mpmc_stack : mpmc_stack Σ unboxed) :=
+  ws_bag_of_spmc_stack (spmc_stack_of_mpmc_stack mpmc_stack).
+
+Class WsBagOfSpmcQueueG Σ `{!heapGS Σ} := {
+  ws_bag_of_spmc_queue_G_model_G : AuthExclG Σ (listO valO) ;
+}.
+#[local] Existing Instance ws_bag_of_spmc_queue_G_model_G.
 
 Definition ws_bag_of_spmc_queue_Σ := #[
   auth_excl_Σ (listO valO)
@@ -625,8 +686,11 @@ Proof.
 Qed.
 
 Section ws_bag_of_spmc_queue.
-  Context `{WsBagOfSpmcQueueG Σ} (spmc_queue : spmc_queue Σ).
-  Implicit Types γ : spmc_queue.(spmc_queue_name) * gname.
+  Context `{WsBagOfSpmcQueueG Σ} {unboxed} (spmc_queue : spmc_queue Σ unboxed).
+
+  Definition ws_bag_of_spmc_queue_name : Type :=
+    spmc_queue.(spmc_queue_name) * gname.
+  Implicit Types γ : ws_bag_of_spmc_queue_name.
 
   Notation "γ .(base)" := γ.1
   ( at level 5
@@ -635,7 +699,7 @@ Section ws_bag_of_spmc_queue.
   ( at level 5
   ) : stdpp_scope.
 
-  Notation ws_bag_of_spmc_queue_meta_ctl := (nroot .@ "ctl").
+  Notation ws_bag_of_spmc_queue_meta_model := (nroot .@ "model").
 
   Notation ws_bag_of_spmc_queue_namespace_base ι := (ι .@ "base").
   Notation ws_bag_of_spmc_queue_namespace_extra ι := (ι .@ "extra").
@@ -656,14 +720,14 @@ Section ws_bag_of_spmc_queue.
       let: "o" := spmc_queue.(spmc_queue_pop) "t" in
       "o".
 
-  #[local] Definition ws_bag_of_spmc_queue_ctl₁ γ vs :=
+  #[local] Definition ws_bag_of_spmc_queue_model₁ γ vs :=
     auth_excl_frag γ.(extra) vs.
-  #[local] Definition ws_bag_of_spmc_queue_ctl₂ γ vs :=
+  #[local] Definition ws_bag_of_spmc_queue_model₂ γ vs :=
     auth_excl_auth γ.(extra) (DfracOwn 1) vs.
 
   #[local] Definition ws_bag_of_spmc_queue_inv_inner γ Ψ : iProp Σ :=
     ∃ vs,
-    ws_bag_of_spmc_queue_ctl₁ γ vs ∗
+    ws_bag_of_spmc_queue_model₁ γ vs ∗
     [∗ list] v ∈ vs, Ψ v.
   #[local] Definition ws_bag_of_spmc_queue_inv t γ ι Ψ : iProp Σ :=
     spmc_queue.(spmc_queue_inv) t γ.(base) (ws_bag_of_spmc_queue_namespace_base ι) ∗
@@ -672,7 +736,7 @@ Section ws_bag_of_spmc_queue.
   #[local] Definition ws_bag_of_spmc_queue_model t γ sz : iProp Σ :=
     ∃ vs,
     ⌜sz = length vs⌝ ∗
-    ws_bag_of_spmc_queue_ctl₂ γ vs ∗
+    ws_bag_of_spmc_queue_model₂ γ vs ∗
     spmc_queue.(spmc_queue_model) t γ.(base) vs.
 
   #[local] Definition ws_bag_of_spmc_queue_owner t γ :=
@@ -725,8 +789,8 @@ Section ws_bag_of_spmc_queue.
     iIntros "%Φ _ HΦ".
     iApply wp_fupd.
     wp_apply (spmc_queue_make_spec with "[//]"). iIntros "%t %γ_deque (#Hinv_deque & Hmodel_deque & Howner)".
-    iMod (auth_excl_alloc' []) as "(%γ_extra & Hctl₂ & Hctl₁)".
-    iApply ("HΦ" $! t (γ_deque, γ_extra)). iFrame. iSplitL "Hctl₁".
+    iMod (auth_excl_alloc' []) as "(%γ_extra & Hmodel₂ & Hmodel₁)".
+    iApply ("HΦ" $! t (γ_deque, γ_extra)). iFrame. iSplitL "Hmodel₁".
     - iFrame "#". iApply inv_alloc. iNext. iExists []. iFrame. done.
     - iExists []. auto with iFrame.
   Qed.
@@ -747,18 +811,18 @@ Section ws_bag_of_spmc_queue.
   Proof.
     iIntros "!> %Φ ((#Hinv_deque & #Hinv_extra) & Howner & Hv) HΦ".
     awp_apply (spmc_queue_push_spec with "[$Hinv_deque $Howner]").
-    iInv "Hinv_extra" as "(%vs & >Hctl₁ & Hvs)".
+    iInv "Hinv_extra" as "(%vs & >Hmodel₁ & Hvs)".
     iApply (aacc_aupd_commit with "HΦ"); first solve_ndisj.
-    iIntros "%sz (%_vs & -> & Hctl₂ & Hmodel_deque)".
-    iDestruct (auth_excl_both_agree_L with "Hctl₂ Hctl₁") as %->.
+    iIntros "%sz (%_vs & -> & Hmodel₂ & Hmodel_deque)".
+    iDestruct (auth_excl_both_agree_L with "Hmodel₂ Hmodel₁") as %->.
     iAaccIntro with "Hmodel_deque".
-    - iIntros "Hmodel_deque !>". iSplitL "Hctl₂ Hmodel_deque".
+    - iIntros "Hmodel_deque !>". iSplitL "Hmodel₂ Hmodel_deque".
       { iExists vs. auto with iFrame. }
       iIntros "$ !>". iFrame. iExists vs. auto with iFrame.
     - set vs' := v :: vs.
       iIntros "Hmodel_deque".
-      iMod (auth_excl_update' vs' with "Hctl₂ Hctl₁") as "(Hctl₂ & Hctl₁)".
-      iModIntro. iSplitL "Hctl₂ Hmodel_deque".
+      iMod (auth_excl_update' vs' with "Hmodel₂ Hmodel₁") as "(Hmodel₂ & Hmodel₁)".
+      iModIntro. iSplitL "Hmodel₂ Hmodel_deque".
       { iExists vs'. auto with iFrame. }
       iIntros "$ !>". iExists vs'. auto with iFrame.
   Qed.
@@ -782,28 +846,28 @@ Section ws_bag_of_spmc_queue.
     iIntros "!> %Φ ((#Hinv_deque & #Hinv_extra) & Howner) HΦ".
     wp_rec.
     awp_apply (spmc_queue_pop_spec with "Hinv_deque").
-    iInv "Hinv_extra" as "(%vs & >Hctl₁ & Hvs)".
+    iInv "Hinv_extra" as "(%vs & >Hmodel₁ & Hvs)".
     iApply (aacc_aupd_commit with "HΦ"); first solve_ndisj.
-    iIntros "%sz (%_vs & -> & Hctl₂ & Hmodel_deque)".
-    iDestruct (auth_excl_both_agree_L with "Hctl₂ Hctl₁") as %->.
+    iIntros "%sz (%_vs & -> & Hmodel₂ & Hmodel_deque)".
+    iDestruct (auth_excl_both_agree_L with "Hmodel₂ Hmodel₁") as %->.
     iAaccIntro with "Hmodel_deque".
-    - iIntros "Hmodel_deque !>". iSplitL "Hctl₂ Hmodel_deque".
+    - iIntros "Hmodel_deque !>". iSplitL "Hmodel₂ Hmodel_deque".
       { iExists vs. auto with iFrame. }
       iIntros "$ !>". iFrame. iExists vs. iFrame.
     - iIntros "%o [((-> & ->) & Hmodel_deque) | (%vs' & %v & (-> & ->) & Hmodel_deque)]".
-      + iModIntro. iExists None. iSplitL "Hctl₂ Hmodel_deque".
+      + iModIntro. iExists None. iSplitL "Hmodel₂ Hmodel_deque".
         { iLeft. iSplit; first done. iExists []. auto with iFrame. }
-        iIntros "HΦ !>". iFrame. iSplitL "Hctl₁ Hvs".
+        iIntros "HΦ !>". iFrame. iSplitL "Hmodel₁ Hvs".
         { iExists []. auto. }
         iIntros "_". wp_pures. iApply "HΦ". auto with iFrame.
-      + iMod (auth_excl_update' vs' with "Hctl₂ Hctl₁") as "(Hctl₂ & Hctl₁)".
+      + iMod (auth_excl_update' vs' with "Hmodel₂ Hmodel₁") as "(Hmodel₂ & Hmodel₁)".
         iDestruct "Hvs" as "(Hvs' & Hv & _)".
-        iModIntro. iExists (Some v). iSplitL "Hctl₂ Hmodel_deque".
+        iModIntro. iExists (Some v). iSplitL "Hmodel₂ Hmodel_deque".
         { iRight. iExists (length vs'), v. iSplit.
           { rewrite app_length (comm Nat.add) //. }
           iExists vs'. auto with iFrame.
         }
-        iIntros "HΦ !>". iSplitL "Hctl₁ Hvs'".
+        iIntros "HΦ !>". iSplitL "Hmodel₁ Hvs'".
         { iExists vs'. auto with iFrame. }
         iIntros "_". wp_pures. iApply "HΦ". auto with iFrame.
   Qed.
@@ -825,37 +889,90 @@ Section ws_bag_of_spmc_queue.
     iIntros "!> %Φ (#Hinv_deque & #Hinv_extra) HΦ".
     wp_rec.
     awp_apply (spmc_queue_pop_spec with "Hinv_deque").
-    iInv "Hinv_extra" as "(%vs & >Hctl₁ & Hvs)".
+    iInv "Hinv_extra" as "(%vs & >Hmodel₁ & Hvs)".
     iApply (aacc_aupd_commit with "HΦ"); first solve_ndisj.
-    iIntros "%sz (%_vs & -> & Hctl₂ & Hmodel_deque)".
-    iDestruct (auth_excl_both_agree_L with "Hctl₂ Hctl₁") as %->.
+    iIntros "%sz (%_vs & -> & Hmodel₂ & Hmodel_deque)".
+    iDestruct (auth_excl_both_agree_L with "Hmodel₂ Hmodel₁") as %->.
     iAaccIntro with "Hmodel_deque".
-    - iIntros "Hmodel_deque !>". iSplitL "Hctl₂ Hmodel_deque".
+    - iIntros "Hmodel_deque !>". iSplitL "Hmodel₂ Hmodel_deque".
       { iExists vs. auto with iFrame. }
       iIntros "$ !>". iExists vs. auto with iFrame.
     - iIntros "%o [((-> & ->) & Hmodel_deque) | (%vs' & %v & (-> & ->) & Hmodel_deque)]".
-      + iModIntro. iExists None. iSplitL "Hctl₂ Hmodel_deque".
+      + iModIntro. iExists None. iSplitL "Hmodel₂ Hmodel_deque".
         { iLeft. iSplit; first done. iExists []. auto with iFrame. }
-        iIntros "HΦ !>". iFrame. iSplitL "Hctl₁ Hvs".
+        iIntros "HΦ !>". iFrame. iSplitL "Hmodel₁ Hvs".
         { iExists []. auto. }
         iIntros "_". wp_pures. iApply "HΦ". auto.
-      + iMod (auth_excl_update' vs' with "Hctl₂ Hctl₁") as "(Hctl₂ & Hctl₁)".
+      + iMod (auth_excl_update' vs' with "Hmodel₂ Hmodel₁") as "(Hmodel₂ & Hmodel₁)".
         iDestruct "Hvs" as "(Hvs' & Hv & _)".
-        iModIntro. iExists (Some v). iSplitL "Hctl₂ Hmodel_deque".
+        iModIntro. iExists (Some v). iSplitL "Hmodel₂ Hmodel_deque".
         { iRight. iExists (length vs'), v. iSplit.
           { rewrite app_length (comm Nat.add) //. }
           iExists vs'. auto with iFrame.
         }
-        iIntros "HΦ !>". iSplitL "Hctl₁ Hvs'".
+        iIntros "HΦ !>". iSplitL "Hmodel₁ Hvs'".
         { iExists vs'. auto with iFrame. }
         iIntros "_". wp_pures. iApply "HΦ". auto with iFrame.
   Qed.
-
-  Definition ws_bag_of_spmc_queue :=
-    Build_ws_bag
-      ws_bag_of_spmc_queue_owner_exclusive
-      ws_bag_of_spmc_queue_make_spec
-      ws_bag_of_spmc_queue_push_spec
-      ws_bag_of_spmc_queue_pop_spec
-      ws_bag_of_spmc_queue_steal_spec.
 End ws_bag_of_spmc_queue.
+
+#[local] Lemma ws_bag_of_spmc_queue_unboxed `{WsBagOfSpmcQueueG Σ} {unboxed} (spmc_queue : spmc_queue Σ unboxed) :
+  if unboxed then ∀ t γ ι Ψ,
+    ws_bag_of_spmc_queue_inv spmc_queue t γ ι Ψ -∗
+    ⌜val_is_unboxed t⌝
+  else
+    True.
+Proof.
+  destruct unboxed; last done.
+  iIntros "%t %γ %ι %Ψ (#Hinv_deque & #Hinv_extra)".
+  iApply (spmc_queue.(spmc_queue_unboxed) with "Hinv_deque").
+Qed.
+
+Definition ws_bag_of_spmc_queue `{WsBagOfSpmcQueueG Σ} {unboxed} (spmc_queue : spmc_queue Σ unboxed) : ws_bag Σ unboxed := {|
+  ws_bag_make := ws_bag_of_spmc_queue_make spmc_queue ;
+  ws_bag_push := ws_bag_of_spmc_queue_push spmc_queue ;
+  ws_bag_pop := ws_bag_of_spmc_queue_pop spmc_queue ;
+  ws_bag_steal := ws_bag_of_spmc_queue_steal spmc_queue ;
+
+  ws_bag_name := ws_bag_of_spmc_queue_name spmc_queue ;
+  ws_bag_inv := ws_bag_of_spmc_queue_inv spmc_queue ;
+  ws_bag_model := ws_bag_of_spmc_queue_model spmc_queue ;
+  ws_bag_owner := ws_bag_of_spmc_queue_owner spmc_queue ;
+
+  ws_bag_inv_ne := ws_bag_of_spmc_queue_inv_ne spmc_queue ;
+  ws_bag_inv_persistent := ws_bag_of_spmc_queue_inv_persistent spmc_queue ;
+  ws_bag_model_timeless := ws_bag_of_spmc_queue_model_timeless spmc_queue ;
+  ws_bag_owner_timeless := ws_bag_of_spmc_queue_owner_timeless spmc_queue ;
+
+  ws_bag_owner_exclusive := ws_bag_of_spmc_queue_owner_exclusive spmc_queue ;
+
+  ws_bag_make_spec := ws_bag_of_spmc_queue_make_spec spmc_queue ;
+  ws_bag_push_spec := ws_bag_of_spmc_queue_push_spec spmc_queue ;
+  ws_bag_pop_spec := ws_bag_of_spmc_queue_pop_spec spmc_queue ;
+  ws_bag_steal_spec := ws_bag_of_spmc_queue_steal_spec spmc_queue ;
+
+  ws_bag_unboxed := ws_bag_of_spmc_queue_unboxed spmc_queue ;
+|}.
+
+Class WsBagOfMpmcQueueG Σ `{!heapGS Σ} := {
+  ws_bag_of_mpmc_queue_G_mpmc_queue_G : SpmcQueueOfMpmcQueueG Σ ;
+  ws_bag_of_mpmc_queue_G_spmc_queue_G : WsBagOfSpmcQueueG Σ ;
+}.
+#[local] Existing Instance ws_bag_of_mpmc_queue_G_mpmc_queue_G.
+#[local] Existing Instance ws_bag_of_mpmc_queue_G_spmc_queue_G.
+
+Definition ws_bag_of_mpmc_queue_Σ := #[
+  spmc_queue_of_mpmc_queue_Σ ;
+  ws_bag_of_spmc_queue_Σ
+].
+Lemma subG_ws_bag_of_mpmc_queue_Σ Σ `{!heapGS Σ} :
+  subG ws_bag_of_mpmc_queue_Σ Σ →
+  WsBagOfMpmcQueueG Σ.
+Proof.
+  pose subG_spmc_queue_of_mpmc_queue_Σ.
+  pose subG_ws_bag_of_spmc_queue_Σ.
+  solve_inG.
+Qed.
+
+Definition ws_bag_of_mpmc_queue `{WsBagOfMpmcQueueG Σ} {unboxed} (mpmc_queue : mpmc_queue Σ unboxed) :=
+  ws_bag_of_spmc_queue (spmc_queue_of_mpmc_queue mpmc_queue).
